\subsection{Ableitungsregeln \color{red}S445,450, erste Seite, zweit letzte Seite}
	\vspace{-2mm}										%TODO_1: Spacing multicols global ändern
	\begin{multicols}{2}
		Linearität: $\left(f(x) + g(x)\right)^{'} = f'(x) + g'(x)$\\
		Produktregel: $(f \cdot g)' = f' g + f g'$\\
		Quotientenregel $\enbrace{\frac{f}{g}}' = \frac{f'g - fg'}{g^2}$\\
		Kettenregel: $\left( f(g(x)) \right)' = f'(g(x)) \cdot g'(x)$\\
		Kehrwertregel: $\left( \frac{1}{f(x)} \right)^{'} = \frac{-f'(x)}{[f(x)]^{2}}$\\
		Konstantenregel: $ \frac{d}{dx}(c) = 0 \quad (c \in \mathbb{R})$
	\end{multicols}
		
		Potenzreihe: $f: ] \underbrace{-R+a, a+R}_{\subseteq D}	 [ \rightarrow \mathbb R, f(x) = \sum_{n=0}^{\infty} a_n (x -a)^n$ \quad $\Rightarrow$ \quad $f'(x) = \sum_{n=0}^{\infty} n a_{n} (x-a)^{n-1}$\\
		\textbf{Tangentengleichung:} $y=f(x_0)+f'(x_0)(x-x_0)$
		
\vspace{1mm}
\hrule
%-------------------------------------------------------------------------------------------------------------------------------------------------
		
\subsection{Integrationsregeln \color{red}S493ff, 1083ff}
	\vspace{-2mm}										%TODO_1
	\begin{multicols}{2}	
		Summenregel:
		$ \int{\left(f(x) + g(x) \right)} dx = \int f(x) dx + \int g(x) dx $ \\[1mm]
		Faktorregel:
		$ \int n \cdot f(x) dx = n \cdot \int f(x) dx $ \\[1mm]
		Potenzregel:
		$ \int x^n dx = \frac{1}{n+1} \cdot x^{n+1} + C  \qquad \quad (n \neq (-1))$\\
	\end{multicols}

		\vspace{1mm}
\hrule
%-------------------------------------------------------------------------------------------------------------------------------------------------

		
\subsection{Wichtige Zahlen}
	$ \sqrt{2} = 1.41421 \quad \sqrt{3} = 1.73205 \quad \sqrt{5} = 2.23607 \quad\sqrt{7} = 2.64575$ \quad
	$ \pi = 3.14159 \quad e = 2.71828 \quad e^{-1} = 0.36788 $
	